theories/CompilerTests.v
@@ -6,45 +6,18 @@ From Vcpu Require Import Plugin.
 Set Printing Width 120.
 Set Printing Depth 10000.
 
-(* Eval hnf in (4 : nat). *)
-
-(* Check (∀ x : _, _) _. *)
-
-Check 5.
-
-Print inl.
-About sum.
-About list.
-
-(* Test. *)
-
 (* Set Printing All. *)
 (* Set Printing Implicit. *)
 
-Print prod.
-
+Vcpu Derive Encoder for unit as unit.
 Vcpu Derive Encoder for prod as prod.
-Print prod_encode.
-
 Vcpu Derive Encoder for bool as bool.
-
 Vcpu Derive Encoder for sum as sum.
-Check sum_len.
-Check sum_encode.
+Vcpu Derive Encoder for option as option.
 
 Vcpu Derive Encoder for (sum bool bool).
 
-Vcpu Derive Encoder for option as option.
-
-(* Vcpu Derive Encoder for vector. *)
-
-Check @option_map.
-Check @pair.
-Check @inl.
-
 Definition identity A (x : A) := x.
-
-Check Nat.add_comm 2 3.
 
 Definition swap A n m (v : vector A (n + m)) : vector A (m + n) :=
   rew [λ k, vector A k] (Nat.add_comm n m) in v.
@@ -53,25 +26,6 @@ Inductive vec' A (n : nat) := vec'_b (a : A).
 
 Definition swap' A n m (v : vec' A (n + m)) : vec' A (m + n) :=
   rew [λ k, vec' A k] (Nat.add_comm n m) in v.
-
-(* Set Printing All. *)
-
-(* negb : bool → bool *)
-(* ->   : ∀ in_len, circuit in_len 1 → circuit in_len 1 *)
-(* ->   : ∀ in_len, bool * circuit in_len 1 → bool * circuit in_len 1 *)
-
-(* @option_map A B : (A → B) → (option A → option B) *)
-(* ->              : ∀ in_len, (circuit in_len A_len → circuit in_len B_len) → circuit in_len (1 + A_len) → circuit in_len (1 + B_len) *)
-
-Compute swap'.
-
-About eq_trans.
-
-Print bool_encode.
-Compute bool_encode true.
-Compute [|true|] +||+ [||] +||+ [||].
-
-Print xorb.
 
 Definition exchange A B (p : A * B) : B * A :=
   match p with
@@ -104,26 +58,87 @@ Fixpoint flip_s (b : bool) n (s : bool) :=
   | S n' => xorb s (flip_s b n' s)
   end.
 
-(* Vcpu Derive Compilation for identity with (F T (F R T)) as identity. *)
-(* Vcpu Derive Compilation for @option_map with (F T (F T (F (F T T) (F T T)))) as option_map. *)
-(* Vcpu Derive Compilation for (λ A : Type, true) with (F T T). *)
-(* Vcpu Derive Compilation for @pair with (F T (F T (F T (F T T)))). *)
-(* Vcpu Derive Compilation for (@inl bool) with (F T (F T T)). *)
-(* Vcpu Derive Compilation for (@pair bool bool true) with (F T T). *)
+Fixpoint vec A n : Type :=
+  match n with
+  | 0 => unit
+  | S n' => A * vec A n'
+  end.
+
+Fixpoint vec_len A A_len (A_encode : A → vector bool A_len) n : nat :=
+  match n with
+  | 0 =>
+    unit_len
+  | S n' =>
+    prod_len A A_len A_encode (vec A n') (vec_len A A_len A_encode n') (λ _, vector_repeat false _)
+  end.
+
+Fixpoint vec_encode A A_len (A_encode : A → vector bool A_len) n : vec A n → vector bool (vec_len A A_len A_encode n) :=
+  match n return vec A n → vector bool (vec_len A A_len A_encode n) with
+  | 0 => λ v,
+    unit_encode v
+  | S n' => λ v,
+    prod_encode A A_len A_encode (vec A n') (vec_len A A_len A_encode n') (vec_encode A A_len A_encode n') v
+  end.
+
+Register vec as vcpu.vec.type.
+Register vec_len as vcpu.vec.len.
+Register vec_encode as vcpu.vec.encode.
+
+Vcpu Derive Encoder for (vec bool ?[n]).
+
+Fixpoint bv_not n : vec bool n → vec bool n :=
+  match n return vec bool n → vec bool n with
+  | 0 => λ '(tt),
+    tt
+  | S n' => λ '(b, bv'),
+    let not_bv' := bv_not n' bv' in
+    (negb b, not_bv')
+  end.
+
+Fixpoint bv_add n : vec bool n → vec bool n → bool * vec bool n :=
+  match n return vec bool n → vec bool n → bool * vec bool n with
+  | 0 => λ bv_1 bv_2,
+    let 'tt := bv_1 in
+    let 'tt := bv_2 in
+    (false, tt)
+  | S n' => λ bv_1 bv_2,
+    let '(b_1, bv_1') := bv_1 in
+    let '(b_2, bv_2') := bv_2 in
+    let carry_in_add_bv_1'_bv_2' := bv_add n' bv_1' bv_2' in
+    let '(carry_in, add_bv_1'_bv_2') := carry_in_add_bv_1'_bv_2' in
+    let b_res := xorb (xorb b_1 b_2) carry_in in
+    let carry_out := (b_1 && b_2) || (carry_in && (b_1 || b_2)) in
+    (carry_out, (b_res, add_bv_1'_bv_2'))
+  end.
+
+Compute bv_add 4 (false, (true, (false, (true, tt)))) (false, (true, (true, (false, tt)))).
+
+(* Check λ input_len input_encode,
+. *)
+
+Vcpu Derive Compilation for identity with (F T (F R T)) as identity.
+Vcpu Derive Compilation for @option_map with (F T (F T (F (F T T) (F T T)))) as option_map.
+Vcpu Derive Compilation for (λ A : Type, true) with (F T T).
+Vcpu Derive Compilation for @pair with (F T (F T (F T (F T T)))).
+Vcpu Derive Compilation for (@inl bool) with (F T (F T T)).
+Vcpu Derive Compilation for (@pair bool bool true) with (F T T).
 (* Vcpu Derive Compilation for swap' with (F T (F R (F R (F T T)))). *)
-(* Vcpu Derive Compilation for (λ b : bool, if b then false else true) with (F R T). *)
-(* Vcpu Derive Compilation for (λ b : bool, if b then false else true) with (F T T). *)
-(* Vcpu Derive Compilation for @fst with (F T (F T (F T T))). *)
-(* Vcpu Derive Compilation for @snd with (F T (F T (F T T))). *)
+Vcpu Derive Compilation for (λ b : bool, if b then false else true) with (F R T).
+Vcpu Derive Compilation for (λ b : bool, if b then false else true) with (F T T).
+Vcpu Derive Compilation for @fst with (F T (F T (F T T))).
+Vcpu Derive Compilation for @snd with (F T (F T (F T T))).
 Vcpu Derive Compilation for negb with (F T T) as negb.
-(* Vcpu Derive Compilation for xorb with (F T (F T T)). *)
-(* Vcpu Derive Compilation for andb with (F T (F T T)). *)
-(* Vcpu Derive Compilation for exchange with (F T (F T (F T T))) as exchange. *)
-(* Vcpu Derive Compilation for (λ p : bool * bool, let (b_1, b_2) := p in b_1 && b_2) with (F T T). *)
-(* Vcpu Derive Compilation for many_things_transform with (F T T) as many_things_transform. *)
-(* Vcpu Derive Compilation for (λ b : bool, let b' := negb b in (b', xorb b' b)) with (F T T). *)
+Vcpu Derive Compilation for andb with (F T (F T T)) as andb.
+Vcpu Derive Compilation for orb with (F T (F T T)) as orb.
+Vcpu Derive Compilation for xorb with (F T (F T T)) as xorb.
+Vcpu Derive Compilation for exchange with (F T (F T (F T T))) as exchange.
+Vcpu Derive Compilation for (λ p : bool * bool, let (b_1, b_2) := p in b_1 && b_2) with (F T T).
+Vcpu Derive Compilation for many_things_transform with (F T T) as many_things_transform.
+Vcpu Derive Compilation for (λ b : bool, let b' := negb b in (b', xorb b' b)) with (F T T).
 Vcpu Derive Compilation for flip with (F T (F R T)) as flip.
-(* Vcpu Derive Compilation for flip_s with (F T (F R (F T T))) as flip_s. *)
+Vcpu Derive Compilation for flip_s with (F T (F R (F T T))) as flip_s.
+Vcpu Derive Compilation for bv_not with (F R (F T T)) as bv_not.
+(* Vcpu Derive Compilation for bv_add with (F R (F T (F T T))) as bv_add. *)
 
 Print negb_orig.
 Print negb_circuit.
@@ -131,3 +146,320 @@ Print negb_wf_circuit.
 Print negb_eval_circuit.
 
 Print flip_circuit.
+Check flip_eval_circuit.
+
+(* Print bv_add_orig.
+Print bv_add_circuit.
+About bv_add_eval_circuit.
+About bv_add_wf_circuit. *)
+
+Definition bv_add_orig :=
+  (fix bv_add (n : nat) : vec bool n → vec bool n → bool * vec bool n :=
+    match n as n0 return (vec bool n0 → vec bool n0 → bool * vec bool n0) with
+    | 0 => λ bv_1 bv_2 : unit, let 'tt := bv_1 in let 'tt := bv_2 in (false, tt)
+    | S n' =>
+        λ bv_1 bv_2 : bool * vec bool n',
+          let
+          '(b_1, bv_1') := bv_1 in
+          let
+          '(b_2, bv_2') := bv_2 in
+            let
+            '(carry_in, add_bv_1'_bv_2') := bv_add n' bv_1' bv_2' in
+            (orb_orig (andb_orig b_1 b_2) (andb_orig carry_in (orb_orig b_1 b_2)),
+              (xorb_orig (xorb_orig b_1 b_2) carry_in, add_bv_1'_bv_2'))
+    end)
+     : ∀ n : nat, vec bool n → vec bool n → bool * vec bool n.
+
+Definition bv_add_circuit :=
+  (λ input_len : nat,
+    fix bv_add_circuit (n : nat) :
+        circuit input_len (vec_len bool bool_len bool_encode n)
+        → circuit input_len (vec_len bool bool_len bool_encode n)
+          → circuit input_len (bool_len + (vec_len bool bool_len bool_encode n + 0)) :=
+      match
+        n as n0
+        return
+          (circuit input_len (vec_len bool bool_len bool_encode n0)
+          → circuit input_len (vec_len bool bool_len bool_encode n0)
+            → circuit input_len (bool_len + (vec_len bool bool_len bool_encode n0 + 0)))
+      with
+      | 0 =>
+          λ _ _ : circuit input_len unit_len,
+            circuit_const input_len
+              ((λ H : bool * unit, let (H0, H1) := H in bool_encode H0 +||+ unit_encode H1 +||+ [||]) (false, tt))
+      | S n' =>
+          λ bv_1_circuit bv_2_circuit : circuit input_len (bool_len + (vec_len bool bool_len bool_encode n' + 0)),
+            circuit_comp
+              (circuit_comp
+                (circuit_comp
+                    (circuit_combine
+                      (circuit_suffix (input_len + (bool_len + (vec_len bool bool_len bool_encode n' + 0)) + bool_len)
+                          bool_len)
+                      (circuit_combine
+                          (circuit_combine
+                            (circuit_comp
+                                (circuit_suffix (input_len + (bool_len + (vec_len bool bool_len bool_encode n' + 0)))
+                                  bool_len)
+                                (circuit_prefix
+                                  (input_len + (bool_len + (vec_len bool bool_len bool_encode n' + 0)) + bool_len)
+                                  bool_len))
+                            (circuit_combine
+                                (circuit_comp
+                                  (circuit_comp
+                                      (circuit_comp_prefix (vec_len bool bool_len bool_encode n') 0
+                                        (circuit_comp_suffix bool_len (vec_len bool bool_len bool_encode n' + 0)
+                                            (circuit_suffix input_len
+                                              (bool_len + (vec_len bool bool_len bool_encode n' + 0)))))
+                                      (circuit_prefix
+                                        (input_len + (bool_len + (vec_len bool bool_len bool_encode n' + 0))) bool_len))
+                                  (circuit_prefix
+                                      (input_len + (bool_len + (vec_len bool bool_len bool_encode n' + 0)) + bool_len)
+                                      bool_len))
+                                (circuit_const
+                                  (input_len + (bool_len + (vec_len bool bool_len bool_encode n' + 0)) + bool_len +
+                                    bool_len)
+                                  [||])))
+                          (circuit_const
+                            (input_len + (bool_len + (vec_len bool bool_len bool_encode n' + 0)) + bool_len + bool_len)
+                            [||])))
+                    (circuit_combine
+                      (circuit_suffix 0
+                          (input_len + (bool_len + (vec_len bool bool_len bool_encode n' + 0)) + bool_len))
+                      (orb_circuit (input_len + (bool_len + (vec_len bool bool_len bool_encode n' + 0)) + bool_len)
+                          (andb_circuit
+                            (input_len + (bool_len + (vec_len bool bool_len bool_encode n' + 0)) + bool_len)
+                            (circuit_comp
+                                (circuit_comp
+                                  (circuit_comp_prefix bool_len (vec_len bool bool_len bool_encode n' + 0)
+                                      bv_1_circuit)
+                                  (circuit_prefix input_len (bool_len + (vec_len bool bool_len bool_encode n' + 0))))
+                                (circuit_prefix (input_len + (bool_len + (vec_len bool bool_len bool_encode n' + 0)))
+                                  bool_len))
+                            (circuit_comp
+                                (circuit_comp
+                                  (circuit_comp_prefix bool_len (vec_len bool bool_len bool_encode n' + 0)
+                                      bv_2_circuit)
+                                  (circuit_prefix input_len (bool_len + (vec_len bool bool_len bool_encode n' + 0))))
+                                (circuit_prefix (input_len + (bool_len + (vec_len bool bool_len bool_encode n' + 0)))
+                                  bool_len)))
+                          (andb_circuit
+                            (input_len + (bool_len + (vec_len bool bool_len bool_encode n' + 0)) + bool_len)
+                            (circuit_comp
+                                (circuit_comp_prefix bool_len (vec_len bool bool_len bool_encode n' + 0)
+                                  (circuit_suffix input_len (bool_len + (vec_len bool bool_len bool_encode n' + 0))))
+                                (circuit_prefix (input_len + (bool_len + (vec_len bool bool_len bool_encode n' + 0)))
+                                  bool_len))
+                            (orb_circuit
+                                (input_len + (bool_len + (vec_len bool bool_len bool_encode n' + 0)) + bool_len)
+                                (circuit_comp
+                                  (circuit_comp
+                                      (circuit_comp_prefix bool_len (vec_len bool bool_len bool_encode n' + 0)
+                                        bv_1_circuit)
+                                      (circuit_prefix input_len (bool_len + (vec_len bool bool_len bool_encode n' + 0))))
+                                  (circuit_prefix
+                                      (input_len + (bool_len + (vec_len bool bool_len bool_encode n' + 0))) bool_len))
+                                (circuit_comp
+                                  (circuit_comp
+                                      (circuit_comp_prefix bool_len (vec_len bool bool_len bool_encode n' + 0)
+                                        bv_2_circuit)
+                                      (circuit_prefix input_len (bool_len + (vec_len bool bool_len bool_encode n' + 0))))
+                                  (circuit_prefix
+                                      (input_len + (bool_len + (vec_len bool bool_len bool_encode n' + 0))) bool_len)))))))
+                (circuit_combine
+                    (circuit_suffix 0 (input_len + (bool_len + (vec_len bool bool_len bool_encode n' + 0))))
+                    (xorb_circuit (input_len + (bool_len + (vec_len bool bool_len bool_encode n' + 0)))
+                      (xorb_circuit (input_len + (bool_len + (vec_len bool bool_len bool_encode n' + 0)))
+                          (circuit_comp
+                            (circuit_comp_prefix bool_len (vec_len bool bool_len bool_encode n' + 0) bv_1_circuit)
+                            (circuit_prefix input_len (bool_len + (vec_len bool bool_len bool_encode n' + 0))))
+                          (circuit_comp
+                            (circuit_comp_prefix bool_len (vec_len bool bool_len bool_encode n' + 0) bv_2_circuit)
+                            (circuit_prefix input_len (bool_len + (vec_len bool bool_len bool_encode n' + 0)))))
+                      (circuit_comp_prefix bool_len (vec_len bool bool_len bool_encode n' + 0)
+                          (circuit_suffix input_len (bool_len + (vec_len bool bool_len bool_encode n' + 0)))))))
+              (circuit_combine (circuit_suffix 0 input_len)
+                (bv_add_circuit n'
+                    (circuit_comp_prefix (vec_len bool bool_len bool_encode n') 0
+                      (circuit_comp_suffix bool_len (vec_len bool bool_len bool_encode n' + 0) bv_1_circuit))
+                    (circuit_comp_prefix (vec_len bool bool_len bool_encode n') 0
+                      (circuit_comp_suffix bool_len (vec_len bool bool_len bool_encode n' + 0) bv_2_circuit))))
+      end)
+      : ∀ input_len n : nat,
+          circuit input_len (vec_len bool bool_len bool_encode n)
+          → circuit input_len (vec_len bool bool_len bool_encode n)
+            → circuit input_len (bool_len + (vec_len bool bool_len bool_encode n + 0)).
+
+Axiom bv_add_eval_circuit
+      : ∀ (input_len : nat) (input_encode : vector bool input_len) (n : nat)
+          (H : vec bool n) (H0 : circuit input_len (vec_len bool bool_len bool_encode n)),
+        circuit_wf H0
+        → circuit_eval H0 input_encode = vec_encode bool bool_len bool_encode n H
+          → ∀ (H1 : vec bool n) (H2 : circuit input_len (vec_len bool bool_len bool_encode n)),
+              circuit_wf H2
+              → circuit_eval H2 input_encode = vec_encode bool bool_len bool_encode n H1
+                → circuit_eval (bv_add_circuit input_len n H0 H2) input_encode =
+                  (λ H3 : bool * vec bool n,
+                    let (H4, H5) := H3 in bool_encode H4 +||+ vec_encode bool bool_len bool_encode n H5 +||+ [||])
+                    (bv_add_orig n H H1).
+
+Axiom bv_add_wf_circuit
+  : ∀ (input_len n : nat) (H : circuit input_len (vec_len bool bool_len bool_encode n)),
+      circuit_wf H
+      → ∀ H0 : circuit input_len (vec_len bool bool_len bool_encode n),
+          circuit_wf H0 → circuit_wf (bv_add_circuit input_len n H H0).
+
+Lemma transparent_eq_nat :
+  ∀ {n m : nat},
+  n = m →
+  n = m.
+Proof.
+  intros n m H_n_m. destruct (Nat.eq_dec n m) as [H | H].
+  - apply H.
+  - exfalso. apply H, H_n_m.
+Defined.
+
+Lemma bool_len_def :
+  ∀ n,
+  vec_len bool bool_len bool_encode n = n.
+Proof.
+  intros n. induction n as [| n' IH].
+  - simpl. reflexivity.
+  - simpl. rewrite IH. unfold prod_len, bool_len. lia.
+Defined.
+
+Definition final_bv_add_circuit n : circuit (n + n) (1 + n) :=
+  rew <- [fun m => circuit (n + n) (bool_len + m)] transparent_eq_nat (plus_n_O n) in
+  rew [fun m => circuit (n + n) (bool_len + (m + 0))] transparent_eq_nat (bool_len_def n) in
+    bv_add_circuit (n + n) n
+      (rew <- [fun m => circuit (n + n) m] transparent_eq_nat (bool_len_def n) in circuit_prefix n n)
+      (rew <- [fun m => circuit (n + n) m] transparent_eq_nat (bool_len_def n) in circuit_suffix n n).
+
+Compute (circuit_wires (final_bv_add_circuit 2)).
+Compute circuit_eval (final_bv_add_circuit 4) [|false; true; false; true; false; true; true; false|].
+
+(* From Equations Require Export Equations.
+From Equations Require Export TransparentEquations. *)
+
+Lemma circuit_wf_final_bv_add_circuit :
+  ∀ n,
+  circuit_wf (final_bv_add_circuit n).
+Proof.
+  intros n. unfold final_bv_add_circuit.
+  remember (transparent_eq_nat (plus_n_O n)) as e.
+  destruct (Nat.eq_dec n (n + 0)).
+Abort.
+
+Definition final_bv_add_circuit' n : circuit (vec_len bool bool_len bool_encode n + vec_len bool bool_len bool_encode n) (bool_len + (vec_len bool bool_len bool_encode n + 0)) :=
+  bv_add_circuit (vec_len bool bool_len bool_encode n + vec_len bool bool_len bool_encode n) n (circuit_prefix (vec_len bool bool_len bool_encode n) (vec_len bool bool_len bool_encode n))(circuit_suffix (vec_len bool bool_len bool_encode n) (vec_len bool bool_len bool_encode n)).
+
+Lemma circuit_wf_final_bv_add_circuit' :
+  ∀ n,
+  circuit_wf (final_bv_add_circuit' n).
+Proof.
+  intros n. unfold final_bv_add_circuit'. apply bv_add_wf_circuit.
+  - apply circuit_wf_circuit_prefix.
+  - apply circuit_wf_circuit_suffix.
+Qed.
+
+Fixpoint vec_to_vector {A n} : vec A n → vector A n :=
+  match n with
+  | 0 => λ '(tt), [||]
+  | S n' => λ '(x, v'), x :||: vec_to_vector v'
+  end.
+
+Lemma circuit_eval_final_bv_add_circuit' :
+  ∀ n (bv_1 bv_2 : vec bool (vec_len bool bool_len bool_encode n)),
+  let '(carry, bv_res) := bv_add (vec_len bool bool_len bool_encode n) bv_1 bv_2 in
+  circuit_eval (final_bv_add_circuit' n) (vec_to_vector bv_1 +||+ vec_to_vector bv_2) =
+  [|carry|] +||+ (vec_to_vector bv_res +||+ [||]).
+Proof.
+  intros n bv_1 bv_2. remember ((bv_add (vec_len bool bool_len bool_encode n) bv_1 bv_2)) as bv_res eqn:H_bv_res. destruct bv_res as [carry add_bv_1_bv_2].
+  unfold final_bv_add_circuit'.
+  pose (bv_1' := rew [λ m, vec bool m] transparent_eq_nat (bool_len_def n) in bv_1); pose (bv_2' := rew [λ m, vec bool m] transparent_eq_nat (bool_len_def n) in bv_2).
+  assert (H_1 :
+    circuit_eval
+      (circuit_prefix (vec_len bool bool_len bool_encode n) (vec_len bool bool_len bool_encode n))
+      (vec_to_vector bv_1 +||+ vec_to_vector bv_2) =
+    vec_encode bool bool_len bool_encode n bv_1'
+  ). {
+    rewrite circuit_eval_circuit_prefix. rewrite vector_prefix_vector_app. subst bv_1'.
+    clear - n bv_1. revert bv_1; induction n as [| n' IH]; intros bv_1; admit.
+  }
+  assert (H_2 :
+    circuit_eval
+      (circuit_suffix (vec_len bool bool_len bool_encode n) (vec_len bool bool_len bool_encode n))
+      (vec_to_vector bv_1 +||+ vec_to_vector bv_2) =
+    vec_encode bool bool_len bool_encode n bv_2'
+  ). {
+    rewrite circuit_eval_circuit_suffix. rewrite vector_suffix_vector_app. subst bv_2'.
+    clear - n bv_2. revert bv_2; induction n as [| n' IH]; intros bv_2; admit.
+  }
+  specialize (bv_add_eval_circuit (vec_len bool bool_len bool_encode n + vec_len bool bool_len bool_encode n) (vec_to_vector bv_1 +||+ vec_to_vector bv_2) n bv_1' (circuit_prefix _ _) (circuit_wf_circuit_prefix _ _) H_1 bv_2' (circuit_suffix _ _) (circuit_wf_circuit_suffix _ _) H_2) as H.
+  rewrite H. destruct (bv_add_orig n bv_1' bv_2') as [carry' add_bv_1'_bv_2'].
+  f_equal > [| f_equal].
+  - admit.
+  - admit.
+Admitted.
+
+Fixpoint bv_to_nat (n : nat) (m : nat) : vec bool n → nat :=
+  match n with
+  | 0 => λ tt, m
+  | S n' => λ '(b, bv'), bv_to_nat n' (m * 2 + (if b then 1 else 0)) bv'
+  end.
+
+Compute bv_to_nat 4 0 (false, (true, (false, (true, tt)))).
+
+Lemma bv_to_nat_add :
+  ∀ n m_1 m_2 m_3 m_4 (bv_1 bv_2 : vec bool n),
+  m_1 + m_2 = m_3 + m_4 →
+  bv_to_nat n m_1 bv_1 + bv_to_nat n m_2 bv_2 = bv_to_nat n m_3 bv_1 + bv_to_nat n m_4 bv_2.
+Proof.
+  intros n m_1 m_2 m_3 m_4 bv_1 bv_2 H_m. revert m_1 m_2 m_3 m_4 H_m; induction n as [| n' IH]; intros m_1 m_2 m_3 m_4 H_m.
+  - destruct bv_1 as [], bv_2 as []. simpl. lia.
+  - destruct bv_1 as [b_1 bv_1'], bv_2 as [b_2 bv_2']. simpl.
+    apply IH. lia.
+Qed.
+
+Lemma bv_add_spec :
+  ∀ n m (bv_1 bv_2 : vec bool n),
+  let '(carry, bv_res) := bv_add n bv_1 bv_2 in
+  bv_to_nat n (m * 2 + (if carry then 1 else 0)) bv_res = bv_to_nat n m bv_1 + bv_to_nat n m bv_2.
+Proof.
+  intros n m bv_1 bv_2. revert m; induction n as [| n' IH]; intros m.
+  - destruct bv_1 as [], bv_2 as []. simpl. lia.
+  - destruct bv_1 as [b_1 bv_1'], bv_2 as [b_2 bv_2']. simpl.
+    specialize (IH bv_1' bv_2'). destruct (bv_add n' bv_1' bv_2') as (carry', bv_res').
+    destruct b_1 as [|], b_2 as [|], carry' as [|]; simpl.
+    + rewrite IH. reflexivity.
+    + rewrite IH. reflexivity.
+    + specialize (IH (m * 2)) as IH.
+      specialize (bv_to_nat_add n' ((m * 2 * 2 + 1) + 1) (m * 2) (m * 2 * 2 + 1) (m * 2 + 1) bv_res' bv_1' ltac:(lia)) as H.
+      ltac1:(replace ((m * 2 + 1) * 2 + 0) with (m * 2 * 2 + 1 + 1) by lia). ltac1:(replace (m * 2 + 0) with (m * 2) by lia). lia.
+    + specialize (IH (m * 2)) as IH.
+      specialize (bv_to_nat_add n' (m * 2 * 2 + 1) (m * 2) (m * 2 * 2) (m * 2 + 1) bv_res' bv_1' ltac:(lia)) as H.
+      ltac1:(replace ((m * 2 + 0) * 2 + 1) with (m * 2 * 2 + 1) by lia). ltac1:(replace (m * 2 + 0) with (m * 2) by lia). ltac1:(replace (m * 2 * 2 + 0) with (m * 2 * 2) in IH by lia). lia.
+    + specialize (IH (m * 2)) as IH.
+      specialize (bv_to_nat_add n' (m * 2 * 2 + 1 + 1) (m * 2) (m * 2 * 2 + 1) (m * 2 + 1) bv_res' bv_2' ltac:(lia)) as H.
+      ltac1:(replace ((m * 2 + 1) * 2 + 0) with (m * 2 * 2 + 1 + 1) by lia). ltac1:(replace (m * 2 + 0) with (m * 2) by lia). lia.
+    + specialize (IH (m * 2)) as IH.
+      specialize (bv_to_nat_add n' (m * 2 * 2 + 1) (m * 2) (m * 2 * 2) (m * 2 + 1) bv_res' bv_2' ltac:(lia)) as H.
+      ltac1:(replace ((m * 2 + 0) * 2 + 1) with (m * 2 * 2 + 1) by lia). ltac1:(replace (m * 2 + 0) with (m * 2) by lia). ltac1:(replace (m * 2 * 2 + 0) with (m * 2 * 2) in IH by lia). lia.
+    + rewrite IH. reflexivity.
+    + rewrite IH. reflexivity.
+Qed.
+
+Lemma final_bv_add_circuit'_spec :
+  ∀ n (bv_1 bv_2 : vec bool (vec_len bool bool_len bool_encode n)),
+  let '(carry, bv_res) := bv_add _ bv_1 bv_2 in
+  circuit_eval (final_bv_add_circuit' n) (vec_to_vector bv_1 +||+ vec_to_vector bv_2) =
+  [|carry|] +||+ (vec_to_vector bv_res +||+ [||]) ∧
+  bv_to_nat _ (if carry then 1 else 0) bv_res = bv_to_nat _ 0 bv_1 + bv_to_nat _ 0 bv_2.
+Proof.
+  intros n bv_1 bv_2.
+  specialize (circuit_eval_final_bv_add_circuit' _ bv_1 bv_2) as H_1.
+  specialize (bv_add_spec _ 0 bv_1 bv_2) as H_2.
+  remember ((bv_add (vec_len bool bool_len bool_encode n) bv_1 bv_2)) as bv_res eqn:H_bv_res. destruct bv_res as [carry add_bv_1_bv_2]. split.
+  - auto.
+  - auto.
+Qed.
+
